language_formal/spark2014_semantics/typing.v
@@ -1,24 +1,558 @@
+Require Import LibTactics.
+Require Import semantics.
+Require Import Setoid.
+Require Import Morphisms.
 Require Import values.
 Require Import environment.
 
 (** * Symbol Table *)
 
+Module Entry_type <: Entry.
+
+Inductive type_stored : Type :=
+| BasicType: type -> type_stored
+| ProcType: list parameter_specification -> type_stored.
+
+Definition T:= (mode*type_stored)%type.
+
+End Entry_type.
+
+Module Import TSTACK := ENV(Entry_type).
+Import Entry_type.
+
+
+Inductive type_of_value: val -> type_stored -> Prop :=
+| TV_Int: forall n, type_of_value (Value (Int n)) (BasicType Integer)
+| TV_Bool: forall b, type_of_value (Value (Bool b)) (BasicType Boolean)
+| TV_Proc: forall pb, type_of_value (Procedure pb) (ProcType (procedure_parameter_profile pb)).
+
+
+Scheme Equality for mode.
+
+Lemma beq_mode_iff1 x: mode_beq x x = true.
+Proof.
+  destruct x;simpl;auto.
+Qed.
+
+Lemma beq_mode_iff2 x y: x<>y -> mode_beq x y = false.
+Proof.
+  destruct x;destruct y;simpl;auto;intros;try contradiction.
+  - destruct H. reflexivity.
+  - destruct H. reflexivity.
+  - destruct H. reflexivity.
+Qed.
+
+
+Lemma beq_mode_true_iff : forall x y, mode_beq x y = true <-> x = y.
+Proof.
+  intros x y.
+  destruct (mode_eq_dec x y);subst.
+  - split;intro.
+    + reflexivity.
+    + apply beq_mode_iff1.
+  - split;intro.
+    + apply beq_mode_iff2 in n.
+      rewrite H in n; discriminate.
+    + contradiction.
+Qed.
+
+
+
+Definition beq_parameter_specification (x y:parameter_specification) : bool :=
+  (beq_nat x.(parameter_subtype_mark) y.(parameter_subtype_mark))
+    &&
+    (mode_beq x.(parameter_mode) y.(parameter_mode)).
+
+Definition eq_parameter_specification (x y:parameter_specification) : Prop :=
+  (x.(parameter_subtype_mark) = y.(parameter_subtype_mark))
+    /\ (x.(parameter_mode) = y.(parameter_mode)).
+
+Lemma eq_parameter_specification_correct: forall x y,
+  eq_parameter_specification x y  <-> beq_parameter_specification x y = true.
+Proof.
+  intros x y.
+  unfold eq_parameter_specification,beq_parameter_specification;simpl.
+  rewrite andb_true_iff.
+  rewrite beq_nat_true_iff.
+  rewrite beq_mode_true_iff.
+  reflexivity.
+Qed.
+
+Inductive eq_parameter_specification_list:
+  list parameter_specification -> list parameter_specification -> Prop :=
+| Eq_paramlis_nil: eq_parameter_specification_list nil nil
+| Eq_paramlis_cons: forall x y a b,
+    eq_parameter_specification x y ->
+    eq_parameter_specification_list a b ->
+    eq_parameter_specification_list (x::a) (y::b).
+
+Function beq_parameter_specification_list (x y:list parameter_specification) {struct x}
+: bool :=
+  match x,y with
+    | nil,nil => true
+    | a::x' , b ::y' =>
+      beq_parameter_specification a b &&
+      beq_parameter_specification_list x' y'
+| _,_ => false
+  end.
+
+Lemma beq_parameter_specification_list_iff:
+  forall l1 l2,
+    eq_parameter_specification_list l1 l2 <->
+    beq_parameter_specification_list l1 l2 = true.
+Proof.
+  intros l1 l2.
+  split.
+  - intros h.
+    induction h;simpl;auto.
+    rewrite eq_parameter_specification_correct in H.
+    rewrite H.
+    rewrite IHh.
+    reflexivity.
+  - revert l2.
+    induction l1;intros l2 h;simpl.
+    + functional inversion h;subst.
+      constructor 1.
+    + functional inversion h;subst.
+      constructor 2.
+      * rewrite andb_true_iff in H1.
+        destruct H1.
+        rewrite eq_parameter_specification_correct.
+        assumption.
+      * apply IHl1.
+        rewrite andb_true_iff in H1.
+        destruct H1.
+        assumption.
+Qed.
+
+
+Inductive compatible_type_of_value: val -> type_stored -> Prop :=
+| CTV_Int: forall n, compatible_type_of_value (Value (Int n)) (BasicType Integer)
+| CTV_Bool: forall b, compatible_type_of_value (Value (Bool b)) (BasicType Boolean)
+| CTV_Undef: forall t, compatible_type_of_value (Undefined) (BasicType t)
+| CTV_Proc: forall pb prf,
+              eq_parameter_specification_list prf (procedure_parameter_profile pb) ->
+              compatible_type_of_value (Procedure pb) (ProcType prf).
+
+
+Lemma eq_parameter_specification_refl : reflexive _ eq_parameter_specification.
+Proof.
+  hnf.
+  intros x.
+  hnf.
+  split;reflexivity.
+Qed.
+
+Lemma eq_parameter_specification_sym : symmetric _ eq_parameter_specification.
+Proof.
+  hnf.
+  intros x y.
+  unfold eq_parameter_specification.
+  intros h.
+  intuition.
+Qed.
+
+Lemma eq_parameter_specification_trans : transitive _ eq_parameter_specification.
+Proof.
+  hnf.
+  intros x y z.
+  unfold eq_parameter_specification.
+  intros h1 h2.
+  intuition.
+  - rewrite H.
+    rewrite H1.
+    reflexivity.
+  - rewrite H0.
+    rewrite H2.
+    reflexivity.
+Qed.
+
+Add Parametric Relation: parameter_specification eq_parameter_specification
+    reflexivity proved by eq_parameter_specification_refl
+    symmetry proved by eq_parameter_specification_sym
+    transitivity proved by eq_parameter_specification_trans
+      as eq_parameter_specification_equiv_rel.
+
+Lemma eq_parameter_specification_list_refl : reflexive _ eq_parameter_specification_list.
+Proof.
+  hnf.
+  induction x.
+  - constructor.
+  - constructor.
+    + reflexivity.
+    + assumption.
+Qed.
+
+Lemma eq_parameter_specification_list_sym : symmetric _ eq_parameter_specification_list.
+Proof.
+  hnf.
+  intros x y H.
+  induction H.
+  - constructor.
+  - constructor.
+    + symmetry.
+      assumption.
+    + assumption.
+Qed.
+
+Lemma eq_parameter_specification_list_trans : transitive _ eq_parameter_specification_list.
+Proof.
+  hnf.
+  intros x y z h.
+  revert z.
+  induction h;intros z h'.
+  - inversion h'.
+    subst.
+    constructor.
+  - inversion h';subst.
+    constructor.
+    + transitivity y;auto.
+    + apply IHh.
+      assumption.
+Qed.
+
+Add Parametric Relation: (list parameter_specification) eq_parameter_specification_list
+    reflexivity proved by eq_parameter_specification_list_refl
+    symmetry proved by eq_parameter_specification_list_sym
+    transitivity proved by eq_parameter_specification_list_trans
+      as eq_parameter_specification_list_equiv_rel.
+
+
+Inductive type_stored_eq : type_stored -> type_stored -> Prop :=
+| TS_eq1: forall x y,
+            eq_parameter_specification_list x y
+            -> type_stored_eq (ProcType x) (ProcType y)
+| TS_eq2: forall x y,
+            x = y
+            -> type_stored_eq (BasicType x) (BasicType y).
+
+
+Lemma type_stored_eq_refl : reflexive _ type_stored_eq.
+Proof.
+  hnf.
+  destruct x.
+  - constructor.
+    reflexivity.
+  - constructor.
+    reflexivity.
+Qed.
+
+Lemma type_stored_eq_sym : symmetric _ type_stored_eq.
+Proof.
+  hnf.
+  intros x y H.
+  destruct H.
+  - constructor.
+    symmetry.
+    assumption.
+  - constructor.
+    symmetry.
+    assumption.
+Qed.
+
+Lemma type_stored_eq_trans : transitive _ type_stored_eq.
+Proof.
+  hnf.
+  intros x y z h.
+  destruct h;intros h'.
+  - inversion h'.
+    subst.
+    constructor.
+    transitivity y;auto.
+  - inversion h';subst.
+    assumption.
+Qed.
+
+Add Parametric Relation: type_stored type_stored_eq
+    reflexivity proved by type_stored_eq_refl
+    symmetry proved by type_stored_eq_sym
+    transitivity proved by type_stored_eq_trans
+      as type_stored_eq_equiv_rel.
+
+
+
+Add Parametric Morphism: 
+  compatible_type_of_value
+    with signature eq ==> type_stored_eq ==> iff
+    as compatible_type_of_value_morph.
+Proof.
+  intros y x y0 H.
+  destruct H.
+  - split.
+    + intros h.
+      inversion h.
+      subst.
+      constructor.
+      transitivity x.
+      * symmetry.
+        assumption.
+      * assumption.
+    + intros h.
+      inv h.
+      constructor.
+      transitivity y0;auto.
+  - subst.
+    reflexivity.
+Qed.
+
+
 (** ** Symbol table as a list *)
 (** it's a map from a variable, represented as natural number,
     to a pair of in/out mode and it's declared type;
 *)
-Definition symtb: Type := list (idnum * (mode * type)).
 
-(** ** Symbol table operations *)
-Fixpoint lookup (x : idnum) (tb: symtb) := 
-   match tb with 
-   | (y, (m,t)) :: tb' => if (beq_nat x y) then Some (m, t) else lookup x tb' 
-   | nil => None
-   end.
+Definition symtb: Type :=  TSTACK.stack.
 
-(** * Type Check Stack *)
+(** * Type Check Store *)
+
+
 
 (** ** Type checker for store *)
+(** A store is a frame of a procedure.
+    for any valid variable x, it has an in/out mode, type and value 
+    (either defined or undefined); as the in/out mode and type are
+    invariant since the variable is declared, and they are used only
+    at compile time, we keep these invariant information in a symbol 
+    table called _symtb_; while the value of a variable will change 
+    as the program executes, and it's used in run time evaluation, 
+    so we keep this information in a store called _store_;
+    
+    Type Check Store means: for any variable x, its stored value in
+    store should be consistent with its declared type recorded in
+    symbol table symtb;
+    
+    This section defines the type checker for store in both relational
+    and functional logic and prove their bisimulation relation
+    - relational one: type_check_store;
+    - functional one: f_type_check_store;
+    - bisilumation proof between relational and functional one;
+*)
+Inductive type_check_store: TSTACK.store -> STACK.store -> Prop :=
+    | TCS_Empty: type_check_store nil nil
+    | TCS_Bool: forall tb s x m b,
+          type_check_store tb s ->
+          type_check_store ((x, (m, BasicType Boolean)) :: tb) ((x, (Value (Bool b))) :: s)
+    | TCS_Int: forall tb s x m v,
+          type_check_store tb s ->
+          type_check_store ((x, (m, BasicType Integer)) :: tb) ((x, (Value (Int v))) :: s)
+    | TCS_Undefined_Bool: forall tb s x m,
+          type_check_store tb s ->
+          type_check_store ((x, (m, BasicType Boolean)) :: tb) ((x, Undefined) :: s)
+    | TCS_Undefined_Int: forall tb s x m,
+          type_check_store tb s ->
+          type_check_store ((x, (m, BasicType Integer)) :: tb) ((x, Undefined) :: s)
+    | TCS_Procedure: forall tb s x m proctype pb ,
+        eq_parameter_specification_list proctype (procedure_parameter_profile pb) ->
+        type_check_store tb s ->
+        type_check_store ((x, (m, ProcType proctype)) :: tb) ((x, Procedure pb) :: s).
+
+
+
+
+Function f_type_check_store (tb: TSTACK.store) (s: STACK.store): bool :=
+    match tb, s with
+    | nil, nil => true
+    | ((x,(m,BasicType Integer)) :: tb'), ((y, (Value (Int _))) :: s')
+    | ((x,(m,BasicType Boolean)) :: tb'), ((y, (Value (Bool _))) :: s') =>
+      if beq_nat x y then f_type_check_store tb' s' else false
+    | ((x,(m,BasicType _)) :: tb'), ((y, Undefined) :: s') => 
+      if beq_nat x y then f_type_check_store tb' s' else false
+    | ((x,(m,ProcType proct)) :: tb'), ((y, Procedure pb) :: s') => 
+      if beq_parameter_specification_list proct (procedure_parameter_profile pb)
+      then
+        if beq_nat x y then f_type_check_store tb' s' else false
+      else false
+    | _, _ => false
+    end.
+
+(** Bisimulation proof between f_type_check_store and type_check_store: 
+    - f_type_check_store_correct
+    - f_type_check_store_complete
+*)
+Lemma f_type_check_store_correct: forall tb s,
+    f_type_check_store tb s = true ->
+        type_check_store tb s.
+Proof.
+    intros tb s.
+    functional induction (f_type_check_store tb s);
+      try rewrite beq_nat_true_iff in *;subst;
+      try now (intros h1;
+               try match goal with
+                     | h: false = true |- _ => inversion h
+                     | h: beq_nat ?x ?y = true |- _ => rewrite (beq_nat_true _ _ e3)
+                   end; constructor; auto).
+
+    - intros h1.
+      destruct _x; constructor;auto.
+    - intros h1.
+      constructor.
+      + apply beq_parameter_specification_list_iff.
+        assumption.
+      + auto.
+Qed.
+
+Lemma f_type_check_store_complete: forall tb s,
+    type_check_store tb s ->
+        f_type_check_store tb s = true.
+Proof.
+    intros tb s h1.
+    induction h1;
+    simpl;
+    repeat match goal with
+    | |- context[beq_nat ?x ?x] => rewrite <- (beq_nat_refl x)
+    | h: f_type_check_store ?tb ?s = true |- _ => rewrite h
+    end; auto.
+    apply beq_parameter_specification_list_iff in H.
+    rewrite H.
+    reflexivity.
+Qed.
+
+
+(* TODO: This is an attempt at giving good names automatically to
+   hypothesis. This is not perfect but should make scripts more
+   robust. This is far from perfect however:
+
+1) I did not manage to make a real tactical, because idify must be
+   undone on hypothesis used by the tactic itself.
+2) rename_norm is not idempotent, which prevents from calling it
+   everywhere.
+ *)
+
+Ltac rename_and_idify H hname :=
+  let th := type of H in
+  rename H into hname;
+  change (id th) in hname;
+  rename_norm;
+  change th in hname
+
+with rename_norm :=
+  match reverse goal with
+    | H: (type_check_store _ _) |- _ =>
+      let s := fresh "htype_check_store" in
+      rename_and_idify H s
+    | H: (beq_nat _ _ = _) |- _ =>
+      let s := fresh "hbeq" in
+      rename_and_idify H s
+    | H: (compatible_type_of_value _ _) |- _ =>
+      let s := fresh "hcompat_t_v" in
+      rename_and_idify H s
+    | H: STACK.fetch _ _ = _ |- _ =>
+      let s := fresh "heqfetch" in
+      rename_and_idify H s
+    | H: STACK.fetchG _ _ = _ |- _ =>
+      let s := fresh "heqfetchG" in
+      rename_and_idify H s
+    | H: fetchG _ _ = _ |- _ =>
+      let s := fresh "heqTfetchG" in
+      rename_and_idify H s
+    | H: fetch _ _ = _ |- _ =>
+      let s := fresh "heqTfetch" in
+      rename_and_idify H s
+    | H: ?f _ _ = _ |- _ =>
+      let s := fresh "heq" f in
+      rename_and_idify H s
+    | _ => idtac
+  end.
+
+Ltac idall :=
+  repeat match goal with
+           | H:_ |- _ =>
+             match type of H with
+               | id _ => fail 1
+               | ?th => change (id th) in H
+             end
+         end.
+
+Ltac unidall :=
+  repeat match goal with
+    | H: id ?th |- _ => change th in H
+  end.
+
+Ltac unid H :=
+  match type of H with
+    | id ?th => change th in H
+  end.
+
+
+
+(* Ltac rename_new tac := *)
+(*   idify_all ltac:(fun x => tac;rename_norm). *)
+Tactic Notation "hhh" tactic(T) := idall; T ; rename_norm ; unidall.
+Tactic Notation "hhh" tactic(T) hyp(h) := idall; unid h; T h ; rename_norm ; unidall.
+
+Tactic Notation "decomp" hyp(h) := idall; unid h; decompose [and ex or] h ; clear h; rename_norm ; unidall.
+
+
+Ltac inv h := idall; unid h; inverts h as;intros; rename_norm;unidall.
+
+(** ** Some lemmas *)
+(** For any variable x in a type checked store, it should has some
+    type t that is compatible with what is in the symbol table;.
+*)
+Lemma type_check_store_spec1:
+  forall tb s x v,
+    type_check_store tb s ->
+    STACK.fetch x s = Some v ->
+    exists t,
+      (compatible_type_of_value v t
+       /\ exists m, TSTACK.fetch x tb = Some (m, t)).
+Proof.
+  intros tb s x v h1 h2.
+  induction h1;functional inversion h2;subst;rename_norm;simpl;try rewrite hbeq;eauto.
+  - exists (BasicType Boolean);split;try constructor;eauto.
+  - exists (BasicType Integer);split;try constructor;eauto.
+  - exists (BasicType Boolean);split;try constructor;eauto.
+  - exists (BasicType Integer);split;try constructor;eauto.
+  - exists (ProcType proctype);split;try constructor;eauto.
+Qed.
+
+
+(** typed_value' means: for any type checked store s with respect to 
+    the symbol table tb, if tb includes a variable x of type t, then 
+    x should also reside in store s, and if x has a defined value v,
+    then v should have the type of t;
+*)
+Lemma type_check_store_spec2: forall tb s x m t,
+    type_check_store tb s ->
+    fetch x tb = Some (m, t) -> 
+    exists v, (STACK.fetch x s = Some v /\ compatible_type_of_value v t).
+Proof.
+    intros tb s x m t h1 h2.
+    induction h1;functional inversion h2;subst;rename_norm
+    ; simpl;try rewrite hbeq;eauto.
+    - exists (Value (Bool b));split;auto;constructor.
+    - exists (Value (Int v));split;auto;constructor.
+    - exists Undefined;split;auto;constructor.
+    - exists Undefined;split;auto;constructor.
+    - exists (Procedure pb);split;auto;constructor.
+      assumption.
+Qed.
+
+
+Lemma type_check_store_spec2_none: forall tb s x,
+    type_check_store tb s ->
+    fetch x tb = None -> 
+    STACK.fetch x s = None.
+Proof.
+  intros tb s x h1 h2.
+  induction h1;functional inversion h2;subst;rename_norm
+    ; simpl;try rewrite hbeq;auto; split;auto;intros v' h;inv h.
+Qed.
+
+Lemma type_check_store_spec1_none:
+  forall tb s x,
+    type_check_store tb s ->
+    STACK.fetch x s = None ->
+    TSTACK.fetch x tb = None.
+Proof.
+  intros tb s x h1 h2.
+  induction h1;functional inversion h2;subst;rename_norm;simpl;try rewrite hbeq;auto.
+Qed.
+
+
+(** * Equality on stacks *)
+
+(** ** Type checker for stack *)
 (** for any valid variable x, it has an in/out mode, type and value 
     (either defined or undefined); as the in/out mode and type are
     invariant since the variable is declared, and they are used only
@@ -37,158 +571,110 @@ Fixpoint lookup (x : idnum) (tb: symtb) :=
     - functional one: f_type_check_store;
     - bisilumation proof between relational and functional one;
 *)
-Inductive type_check_store: symtb -> store -> Prop :=
-    | TC_Empty: type_check_store nil nil
-    | TC_Bool: forall tb s x m b,
-          type_check_store tb s ->
-          type_check_store ((x, (m, Boolean)) :: tb) ((x, (Value (Bool b))) :: s)
-    | TC_Int: forall tb s x m v,
-          type_check_store tb s ->
-          type_check_store ((x, (m, Integer)) :: tb) ((x, (Value (Int v))) :: s)
-    | TC_Undefined_Bool: forall tb s x m,
-          type_check_store tb s ->
-          type_check_store ((x, (m, Boolean)) :: tb) ((x, Undefined) :: s)
-    | TC_Undefined_Int: forall tb s x m,
-          type_check_store tb s ->
-          type_check_store ((x, (m, Integer)) :: tb) ((x, Undefined) :: s).
+Inductive type_check_stack: TSTACK.stack -> STACK.stack -> Prop :=
+    | TCST_nil: type_check_stack nil nil
+    | TCST_cons: forall sto1 sto2 st1 st2,
+                   type_check_store sto1 sto2 ->
+                   type_check_stack st1 st2 ->
+                   type_check_stack (sto1::st1) (sto2::st2).
 
-Function f_type_check_store (tb: symtb) (s: store): bool :=
+
+Function f_type_check_stack (tb: TSTACK.stack) (s: STACK.stack): bool :=
     match tb, s with
     | nil, nil => true
-    | (u :: tb'), (v :: s') => 
-        match u, v with
-        | (x, (m, Boolean)), (y, (Value (Bool b))) => 
-            if beq_nat x y then f_type_check_store tb' s' else false
-        | (x, (m, Integer)), (y, (Value (Int v))) => 
-            if beq_nat x y then f_type_check_store tb' s' else false
-        | (x, (m, Boolean)), (y, Undefined) => 
-            if beq_nat x y then f_type_check_store tb' s' else false
-        | (x, (m, Integer)), (y, Undefined) => 
-            if beq_nat x y then f_type_check_store tb' s' else false
-        | _, _ => false
-        end
-    | _, _ => false
+    | (sto1::st1), (sto2::st2) =>
+      if f_type_check_store sto1 sto2 then
+        f_type_check_stack st1 st2
+      else false
+    | _ , _  => false
     end.
 
 (** Bisimulation proof between f_type_check_store and type_check_store: 
     - f_type_check_store_correct
     - f_type_check_store_complete
 *)
-Lemma f_type_check_store_correct: forall tb s,
-    f_type_check_store tb s = true ->
-        type_check_store tb s.
+Lemma f_type_check_stack_correct: forall tb s,
+    f_type_check_stack tb s = true ->
+        type_check_stack tb s.
 Proof.
     intros tb s.
-    functional induction (f_type_check_store tb s);
-    intros h1;
-    try match goal with
-    | h: false = true |- _ => inversion h
-    | h: beq_nat ?x ?y = true |- _ => rewrite (beq_nat_true _ _ e3)
-    end; constructor; auto.
+    functional induction (f_type_check_stack tb s);intros; try discriminate;rename_norm.
+    - constructor.
+    - constructor;auto.
+      apply f_type_check_store_correct.
+      assumption.
 Qed.
 
-Lemma f_type_check_store_complete: forall tb s,
-    type_check_store tb s ->
-        f_type_check_store tb s = true.
+Lemma f_type_check_stack_complete: forall tb s,
+    type_check_stack tb s ->
+        f_type_check_stack tb s = true.
 Proof.
     intros tb s h1.
-    induction h1;
-    simpl;
-    repeat match goal with
-    | |- context[beq_nat ?x ?x] => rewrite <- (beq_nat_refl x)
-    | h: f_type_check_store ?tb ?s = true |- _ => rewrite h
-    end; auto.
+    induction h1;simpl;auto.
+    rewrite f_type_check_store_complete;auto.
 Qed.
 
-(** ** Some lemmas *)
-(** typed_value means: for any variable x in a type checked store,
-    it should has some type t that can be found in the symbol table;
-*)
-Lemma typed_value: forall tb s x v,
-    type_check_store tb s ->
-    fetch x s = Some (Value v) ->
-    (exists t, value_of_type v t /\ ( exists m, lookup x tb = Some (m, t))).
+
+Lemma type_check_stack_spec1:
+  forall tb s x v,
+    type_check_stack tb s ->
+    STACK.fetchG x s = Some v ->
+    exists t,
+      (compatible_type_of_value v t
+       /\ exists m, TSTACK.fetchG x tb = Some (m, t)).
 Proof.
-    intros tb s x v h1 h2.
-    destruct v.
-  - exists Integer.
-    split.
-    + constructor.
-    + induction h1;
-       [inversion h2 | | | | ];
-       unfold fetch in h2;
-       unfold lookup;
-       destruct (beq_nat x x0);
-       [ inversion h2 | | exists m; auto | | inversion h2 | | inversion h2 | ];
-       fold fetch in h2;
-       fold lookup;
-       specialize (IHh1 h2);
-       assumption.
-  - exists Boolean.
-    split.
-    + constructor.
-    + induction h1;
-       [inversion h2 | | | | ];
-       unfold fetch in h2;
-       unfold lookup;
-       destruct (beq_nat x x0);
-       [ exists m; auto | | inversion h2 | | inversion h2 | | inversion h2 | ];
-       fold fetch in h2;
-       fold lookup;
-       specialize (IHh1 h2);
-       assumption.
+  intros tb s x v h1.
+  revert x v.
+  induction h1;intros x v h2.
+  - functional inversion h2.
+  - functional inversion h2;subst;rename_norm.
+    + apply (type_check_store_spec1 sto1 sto2 x v) in htype_check_store.
+      * decomp htype_check_store;rename_norm;rename_norm.
+        exists x0.
+        split;auto.
+        exists x1.
+        simpl.
+        rewrite heqTfetch.
+        reflexivity.
+      * assumption.      
+    + eapply type_check_store_spec1_none with sto1 sto2 x in htype_check_store;auto.
+      specialize (IHh1 _ _ heqfetchG0).
+      decomp IHh1.
+      exists x0.
+      split;auto.
+      exists x1.
+      simpl.
+      rewrite heqTfetchG.
+      rewrite htype_check_store.
+      reflexivity.
 Qed.
-
-Ltac rm_ex :=
-    repeat match goal with
-    | [ h: exists _, _ |- _ ] => inversion h; clear h
-    | [ h: _ /\ _  |- _ ] => inversion h; clear h
-    end.
-
-Ltac tv_l1 f1 f2 h1 h2 x x0 := 
-    unfold f1 in h1;
-    unfold f2;
-    destruct (beq_nat x x0);
-    [ auto |
-      fold f1 in h1;
-      fold f2;
-      specialize (h2 h1);
-      rm_ex; auto
-    ].
-
-Ltac tv_l2 f1 f2 h1 h2 x x0 tac :=
-    unfold f1 in h1;
-    unfold f2;
-    destruct (beq_nat x x0);
-    [ intros; 
-      inversion h1; subst;
-      inversion H; subst; 
-      tac |
-      fold f1 in h1;
-      fold f2;
-      specialize (h2 h1);
-      rm_ex; auto
-    ].
 
 (** typed_value' means: for any type checked store s with respect to 
     the symbol table tb, if tb includes a variable x of type t, then 
     x should also reside in store s, and if x has a defined value v,
     then v should have the type of t;
 *)
-Lemma typed_value': forall tb s x m t,
-    type_check_store tb s ->
-    lookup x tb = Some (m, t) -> 
-    reside x s = true /\ 
-    (forall v, (Some (Value v) = fetch x s) -> value_of_type v t).
+Lemma type_check_stack_spec2: forall tb s x m t,
+    type_check_stack tb s ->
+    fetchG x tb = Some (m, t) -> 
+    (exists v,  STACK.fetchG x s = Some v /\ compatible_type_of_value v t).
 Proof.
     intros tb s x m t h1 h2.
-    induction h1;
-    [inversion h2 | | | | ];
-    split;
-    [ | tv_l2 lookup fetch h2 IHh1 x x0 constructor |
-      | tv_l2 lookup fetch h2 IHh1 x x0 constructor |
-      | tv_l2 lookup fetch h2 IHh1 x x0 auto |
-      | tv_l2 lookup fetch h2 IHh1 x x0 auto
-    ];
-    tv_l1 lookup reside h2 IHh1 x x0.
-Qed.
+    induction h1;functional inversion h2;subst;rename_norm.
+    - functional inversion heqTfetchG;subst; clear heqTfetchG;rename_norm;rename_norm.
+      + generalize (type_check_store_spec2 _ _ _ _ _ htype_check_store heqTfetch0).
+        intro hh.
+        decomp hh.
+        exists x0;simpl.
+        rewrite heqfetch.
+        auto.
+      + Rinversion fetch.
+    - specialize (IHh1 heqTfetchG0).
+      decomp IHh1.
+      exists x0.
+      simpl.
+      generalize (type_check_store_spec2_none _ _ _ htype_check_store heqTfetch).
+      intros hhh.
+      rewrite hhh.
+      auto.
+Qed.       
